update more examples

FX10.v
@@ -17,104 +17,130 @@ Inductive State := | state (p : program) (A : array) (T : tree).
 
 Inductive stepsto : State -> State -> Prop :=
 | stepsto_1 (p : program) (A : array) (T : tree):
-    stepsto 
-      (state p A (done :> T)) 
+    stepsto
+      (state p A (done :> T))
       (state p A T)
 | stepsto_2 (p : program) (A : array) (T : tree) (A' : array) (T' : tree) (T2 : tree):
-    stepsto 
-      (state p A T) 
-      (state p A' T') 
-    -> 
-    stepsto 
-      (state p A (T :> T2)) 
+    stepsto
+      (state p A T)
+      (state p A' T')
+    ->
+    stepsto
+      (state p A (T :> T2))
       (state p A' (T' :> T2))
 | stepsto_3 (p : program) (A : array) (T : tree):
-    stepsto 
-      (state p A (done || T)) 
+    stepsto
+      (state p A (done || T))
       (state p A T)
 | stepsto_4 (p : program) (A : array) (T : tree):
-    stepsto 
-      (state p A (T || done)) 
+    stepsto
+      (state p A (T || done))
       (state p A T)
 | stepsto_5 (p : program) (A : array) (T : tree) (A' : array) (T' : tree) (T2 : tree):
-    stepsto 
-      (state p A T) 
-      (state p A' T') 
-    -> 
-    stepsto 
-      (state p A (T || T2)) 
+    stepsto
+      (state p A T)
+      (state p A' T')
+    ->
+    stepsto
+      (state p A (T || T2))
       (state p A' (T' || T2))
 | stepsto_6 (p : program) (A : array) (T : tree) (A' : array) (T' : tree) (T2 : tree):
-    stepsto 
-      (state p A T) 
-      (state p A' T') 
-    -> 
-    stepsto 
-      (state p A (T2 || T)) 
+    stepsto
+      (state p A T)
+      (state p A' T')
+    ->
+    stepsto
+      (state p A (T2 || T))
       (state p A' (T2 || T'))
 | stepsto_7 (p : program) (A : array):
-    stepsto 
-      (state p A (statements skip)) 
+    stepsto
+      (state p A (statements skip))
       (state p A done)
 | stepsto_8 (p : program) (A : array) (k : statement):
-    stepsto 
-      (state p A (statements (seq skp k))) 
+    stepsto
+      (state p A (statements (seq skp k)))
       (state p A (statements k))
 | stepsto_9 (p : program) (A : array) (k : statement) (d : nat) (e : expr):
-    stepsto 
-      (state p A (statements (seq (assignment d e) k))) 
+    stepsto
+      (state p A (statements (seq (assignment d e) k)))
       (
-        match e with 
+        match e with
         | const n => (state p (assign A d n) (statements k))
         | incr i => (state p (assign A d ((access A i) + 1)) (statements k))
         end
       )
 | stepsto_10_11 (p : program) (A : array) (k : statement) (d : nat) (s : statement):
-    stepsto 
-      (state p A (statements (seq (while d s) k))) 
+    stepsto
+      (state p A (statements (seq (while d s) k)))
       (
-        match (access A d) with 
+        match (access A d) with
         | O => (state p A (statements k))
         | S n => (state p A (statements (join s (seq (while d s) k))))
         end
       )
 | stepsto_12 (p : program) (A : array) (k : statement) (s : statement):
-    stepsto 
+    stepsto
       (state p A (statements (seq (async s) k)))
       (state p A ((statements s) || (statements k)))
 | stepsto_13 (p : program) (A : array) (k : statement) (s : statement):
-    stepsto 
+    stepsto
       (state p A (statements (seq (finish s) k)))
       (state p A ((statements s) :> (statements k)))
 | stepsto_14 (p : program) (A : array) (k : statement) (s : statement):
-    stepsto 
+    stepsto
       (state p A (statements (seq (call s) k)))
       (state p A (statements (join s k)))
 .
 
-Example test_stepsto1:  
-  stepsto 
-    (state (p {}) (array_init 0) (done :> (statements {skp}))) 
+Example test_stepsto1:
+  stepsto
+    (state (p {}) (array_init 0) (done :> (statements {skp})))
     (state (p {}) (array_init 0) (statements {skp})).
 Proof. apply stepsto_1. Qed.
 
 (* TODO Example test_stepsto2: *)
+Example test_stepsto2:
+    stepsto
+      (state (p {}) (array_init 0) (done :> (statements {skp})))
+      (state (p {}) (array_init 1) (statements {skp}))  ->
+    stepsto
+      (state (p {}) (array_init 0) ((done :> (statements {skp})):> (statements {assignment 0 (const 1)})))
+      (state (p {}) (array_init 1) ((statements {skp}) :> (statements {assignment 0 (const 1)}))).
+Proof. apply stepsto_2. Qed.
 
-Example test_stepsto3:  
-  stepsto 
-    (state (p {}) (array_init 0) (done || (statements {skp}))) 
+Example test_stepsto3:
+  stepsto
+    (state (p {}) (array_init 0) (done || (statements {skp})))
     (state (p {}) (array_init 0) (statements {skp})).
 Proof. apply stepsto_3. Qed.
 
-Example test_stepsto4:  
-  stepsto 
+Example test_stepsto4:
+  stepsto
     (state (p {}) (array_init 0) ((statements {skp}) || done))
     (state (p {}) (array_init 0) (statements {skp})).
 Proof. apply stepsto_4. Qed.
 
-(* TODO Example test_stepsto5: *)
 
-(* TODO Example test_stepsto6: *)
+Example test_stepsto5:
+    stepsto
+      (state (p {}) (array_init 0) (done :> (statements {skp})))
+      (state (p {}) (array_init 0) (done :> (statements {skp})))
+    ->
+    stepsto
+      (state (p {}) (array_init 0) ((done :> (statements {skp})) || (statements {assignment 0 (const 1)})))
+      (state (p {}) (array_init 0) ((done :> (statements {skp})) || (statements {assignment 0 (const 1)}))).
+Proof. apply stepsto_5. Qed.
+
+Definition a0 := state (p {}) (array_init 0).
+Example test_stepsto6:
+    stepsto
+      (state (p {}) (array_init 0) (done :> (statements {skp})))
+      (state (p {}) (array_init 0) (done :> (statements {skp})))
+    ->
+    stepsto
+      (state (p {}) (array_init 0) ((statements {assignment 0 (const 1)}) || (done :> (statements {skp}))))
+      (state (p {}) (array_init 0) ((statements {assignment 0 (const 1)}) || (done :> (statements {skp})))).
+Proof. apply stepsto_6. Qed.
 
 Example test_stepsto7:
   stepsto
@@ -124,19 +150,29 @@ Proof. apply stepsto_7. Qed.
 
 Example test_stepsto8:
   stepsto
-    (state (p {}) (array_init 0) (statements (seq skp (seq (assignment 0 (const 1)) skip) ) ) ) 
+    (state (p {}) (array_init 0) (statements (seq skp (seq (assignment 0 (const 1)) skip) ) ) )
     (state (p {}) (array_init 0) (statements (seq (assignment 0 (const 1)) skip) ) ).
 Proof. apply stepsto_8. Qed.
 
 Example test_stepsto9:
   stepsto
-    (state (p {}) (array_init 1) (statements (seq (assignment 0 (const 1)) skip))) 
+    (state (p {}) (array_init 1) (statements (seq (assignment 0 (const 1)) skip)))
     (state (p {}) ([1]) (statements skip)).
 Proof. apply stepsto_9. Qed.
 
 (* TODO Example test_stepsto10: *)
-
 (* TODO Example test_stepsto11: *)
+Example test_stepsto10_11:
+    stepsto
+      (a0 (statements (seq (while 0 skip) skip)))
+      (
+        match (access (array_init 0) 0) with
+        | O => (state (p {}) (array_init 0) (statements skip))
+        | S n => (state (p {}) (array_init 0) (statements (join skip (seq (while 0 skip) skip))))
+        end
+      ).
+Proof. apply stepsto_10_11. Qed.
+
 
 Example test_stepsto12:
   stepsto
@@ -150,4 +186,10 @@ Example test_stepsto13:
     (state (p {}) (array_init 0) ((statements skip) :> (statements skip))).
 Proof. apply stepsto_13. Qed.
 
-(* TODO Example test_stepsto14: *)
+Example test_stepsto14:
+  stepsto
+    (a0 (statements (seq (call skip) skip)))
+    (a0 (statements (join skip skip))).
+Proof. apply stepsto_14. Qed.
+
+
